git/Izzimach/qinglong/examples/MutexTrack.lean
@@ -1,0 +1,88 @@
+
+--
+-- Index for monads to track mutex locking/unlocking
+--
+
+import QingLong.Data.IndexedMonad
+
+import Lean
+import Lean.Parser
+
+open Lean Elab Command Term Meta 
+open Parser.Term
+
+open IndexedMonad
+
+inductive MutexStep (maxIndex : Nat) where
+| Lock : Fin maxIndex → MutexStep maxIndex
+| Unlock : Fin maxIndex → MutexStep maxIndex
+
+inductive MutexSequence (maxIndex : Nat) where
+| mk : List (MutexStep maxIndex) → MutexSequence maxIndex
+
+instance : Inhabited (MutexSequence mi) where
+    default := MutexSequence.mk []
+
+instance : HAdd (MutexSequence mi) (MutexSequence mi) (MutexSequence mi) where
+    hAdd := fun m1 m2 => match m1,m2 with
+                         | .mk l1 , .mk l2 => .mk (l1 ++ l2)
+
+inductive MutexCommand (maxIndex : Nat) (a : Type) where
+| command : MutexStep maxIndex → MutexCommand maxIndex a
+
+
+variable {n : Nat} {m : Indexer (MutexStep n) → Type → Type 1}
+
+
+def lockMutex [SendableIx (MutexCommand n) m] (i : Fin n)
+  : m (Indexer.Leaf (MutexStep.Lock i)) Unit :=
+    sendIndexed _ (MutexCommand.command (MutexStep.Lock i))
+    
+def unlockMutex [SendableIx (MutexCommand n) m] (i : Fin n) 
+  : m (Indexer.Leaf (MutexStep.Unlock i)) Unit :=
+    sendIndexed _ (MutexCommand.command (MutexStep.Unlock i))
+
+--
+-- Mapping from strings to mutex indices
+--
+-- A better route might be to embed the name list into MutexCommand type and use
+-- existential types to show inclusion, i.e., (MutexCommand (names : ["argh","ack","ugh"]) Unit)
+-- and proofs of the form (∃ i, names[i] = "argh") instead of typeclass instances
+--
+
+class NamedMutex (name : String) (m : Nat) where
+    lockNamed : MutexStep m
+    unlockNamed : MutexStep m
+
+def lockNamedMutex [SendableIx (MutexCommand n) m] [NamedMutex "argh" n] (name : String)
+  : m (Indexer.Leaf (NamedMutex.lockNamed "argh")) Unit :=
+    sendIndexed _ (MutexCommand.command (@NamedMutex.lockNamed "argh" n _))
+
+def unlockNamedMutex [SendableIx (MutexCommand n) m] [NamedMutex "argh" n] (name : String)
+  : m (Indexer.Leaf (NamedMutex.unlockNamed "argh")) Unit :=
+    sendIndexed _ (MutexCommand.command (@NamedMutex.unlockNamed "argh" n _))
+
+
+def elabMutexNames (names : List Syntax) (maxIndex : Nat) (curIndex : Nat) : CommandElabM Unit :=
+    -- this doesn't seem right
+    let maxI : Syntax := Syntax.mkNumLit <| toString maxIndex
+    let curI : Syntax := Syntax.mkNumLit <| toString curIndex
+    match names with
+    | List.nil => pure ()
+    | List.cons h t => do
+        let instanceCmd ←
+          `(instance  : NamedMutex $h $maxI where
+              lockNamed := MutexStep.Lock $curI
+              unlockNamed := MutexStep.Unlock $curI)
+        elabCommand instanceCmd
+        elabMutexNames t maxIndex (curIndex+1)
+
+elab "defineMutexNames" vals:term,+ : command => do
+    let valList := Array.toList (vals : Array Syntax)
+    let maxIndex := List.length valList
+    elabMutexNames valList maxIndex 0
+
+defineMutexNames "argh","ack"
+
+#check @NamedMutex.lockNamed "argh" _ _
+
