git/Izzimach/qinglong/src/QingLong.lean
@@ -1,8 +1,7 @@
 
-import QingLong.Data.OpenUnion
+import QingLong.Data.StateIO
 import QingLong.W.FreerIxW
 
-open openunion
 open FreerIxW
 
 
