git/Izzimach/qinglong/src/QingLong/Eff/Eff.lean
@@ -9,7 +9,7 @@ open Lean Elab Command Term --Meta
 
 open openunion
 
-namespace effW
+namespace Eff
 
 
 
@@ -238,4 +238,4 @@ def runState {α : Type} {effs : List (Type → Type)} {s : Type} (state : s) : 
     fun effVal => handleRelayS state (fun s x => pure (x,s)) stateGo effVal
 
 
-end effW
+end Eff
