git/Izzimach/qinglong/src/QingLong/Macro/FreerIxMacro.lean
@@ -13,9 +13,16 @@ open Parser.Term
 open IndexedMonad
 open SumMacro
 
+
 set_option hygiene false in
 macro "mkFreerInductive" freerName:ident f:ident : command =>
   `(inductive $freerName {ix : Type} (i : Indexer ix) (α : Type u) : Type (u + 1) where 
+      | Pure : α → $freerName i α 
+      | Impure : {x : Type} → $f x → (x → $freerName i α) → $freerName i α)
+
+set_option hygiene false in
+macro "mkFreerInductiveWithIndex" freerName:ident f:ident ix:term : command =>
+  `(inductive $freerName (i : Indexer $ix) (α : Type u) : Type (u + 1) where 
       | Pure : α → $freerName i α 
       | Impure : {x : Type} → $f x → (x → $freerName i α) → $freerName i α)
 
@@ -42,99 +49,147 @@ macro "mkFFunctor" freeName:ident fmapName:ident f:ident : command => do
         map := $fmapName
         )
 
-elab "mkFMonad" freeName:ident bindName:ident f:ident : command => do
+def mkFMonadFunc (freeName : Syntax) (bindName : Syntax) (f :Syntax) (oix : Option Syntax) : CommandElabM Unit := do
   let c1c : Syntax := Lean.mkIdent (freeName.getId ++ "Pure")
   let c2c : Syntax := Lean.mkIdent (freeName.getId ++ "Impure")
   let c1pat ← `(matchAltExpr| | $c1c a => f a)
   let c2pat ← `(matchAltExpr| | $c2c fa next => $c2c fa (fun z => $bindName (next z) f))
   let branches := #[c1pat,c2pat]
-  let bindF ← `(def $bindName {α β ix : Type} {i : Indexer ix} (m : $freeName i α) (f : α → $freeName i β) : $freeName i β := match m with $branches:matchAlt*)
-  elabCommand bindF
+  let matchTerm ← `(match m with $branches:matchAlt*)
+  let bindDecl ← match oix with
+                 | Option.none => `(def $bindName {α β ix : Type} {i : Indexer ix} (m : $freeName i α) (f : α → $freeName i β) : $freeName i β := $matchTerm)
+                 | Option.some ix => `(def $bindName {α β : Type} {i : Indexer $ix} (m : $freeName i α) (f : α → $freeName i β) : $freeName i β := $matchTerm)
+  elabCommand bindDecl
   let monadI ←
-    `(instance {ix : Type} {i : Indexer ix} : Monad ($freeName i) where
-        pure := $c1c
-        bind := $bindName
-        )
+      match oix with
+      | Option.none =>
+            `(instance {ix : Type} {i : Indexer ix} : Monad ($freeName i) where
+                pure := $c1c
+                bind := $bindName)
+      | Option.some ix =>
+            `(instance {i : Indexer $ix} : Monad ($freeName i) where
+                pure := $c1c
+                bind := $bindName)
   elabCommand monadI
 
-elab "mkIxMonad" freeName:ident bindName:ident reindexName:ident f:ident : command => do
+elab "mkFMonad" freeName:ident bindName:ident f:ident : command => mkFMonadFunc freeName bindName f Option.none
+elab "mkFMonad" freeName:ident bindName:ident f:ident ix:term : command => mkFMonadFunc freeName bindName f (Option.some ix)
+
+def mkIxMonadFunc (freeName : Syntax) (bindName : Syntax) (reindexName : Syntax) (f : Syntax) (oix : Option Syntax) : CommandElabM Unit := do
   let c1c : Syntax := Lean.mkIdent (freeName.getId ++ "Pure")
   let c2c : Syntax := Lean.mkIdent (freeName.getId ++ "Impure")
   let reindex1pat ← `(matchAltExpr| | $c1c a => $c1c a)
   let reindex2pat ← `(matchAltExpr| | $c2c fa next => $c2c fa (fun x => $reindexName (next x)))
   let reindexBranches := #[reindex1pat, reindex2pat]
-  let reindexF ← `(def $reindexName {α ix : Type} {i₁ i₂ : Indexer ix} (m : $freeName i₁ α) : $freeName i₂ α := match m with $reindexBranches:matchAlt*)
+  let reindexF ←
+    match oix with
+    | Option.none => `(def $reindexName {α ix : Type} {i₁ i₂ : Indexer ix} (m : $freeName i₁ α) : $freeName i₂ α := match m with $reindexBranches:matchAlt*)
+    | Option.some ix => `(def $reindexName {α : Type} {i₁ i₂ : Indexer $ix} (m : $freeName i₁ α) : $freeName i₂ α := match m with $reindexBranches:matchAlt*)
   elabCommand reindexF
   let c1pat ← `(matchAltExpr| | $c1c a => $reindexName <| f a)
   let c2pat ← `(matchAltExpr| | $c2c fa next => $c2c fa (fun z => $bindName (next z) f))
   let branches := #[c1pat,c2pat]
-  let bindF ← `(def $bindName {α β ix : Type} {i₁ i₂ : Indexer ix} (m : $freeName i₁ α) (f : α → $freeName i₂ β) : $freeName (Indexer.Append i₁ i₂) β := match m with $branches:matchAlt*)
+  let bindF ← 
+    match oix with
+    | Option.none => `(def $bindName {α β ix : Type} {i₁ i₂ : Indexer ix} (m : $freeName i₁ α) (f : α → $freeName i₂ β) : $freeName (Indexer.Append i₁ i₂) β := match m with $branches:matchAlt*)
+    | Option.some ix => `(def $bindName {α β : Type} {i₁ i₂ : Indexer $ix} (m : $freeName i₁ α) (f : α → $freeName i₂ β) : $freeName (Indexer.Append i₁ i₂) β := match m with $branches:matchAlt*)
   elabCommand bindF
   let monadI ←
-    `(instance {ix : Type} : IxMonad (@$freeName ix) where
-        pureIx := fun i a => @$c1c ix i _ a
-        bindIx := $bindName
-        )
+    match oix with
+    | Option.none => 
+        `(instance {ix : Type} : IxMonad (@$freeName ix) where
+            pureIx := fun i a => @$c1c ix i _ a
+            bindIx := $bindName)
+    | Option.some ix => 
+        `(instance : IxMonad $freeName where
+            pureIx := fun i a => @$c1c i _ a
+            bindIx := $bindName)
   elabCommand monadI
 
 
-elab "mkSendableIx" freeName:ident f:ident : command => do
+def mkSendableIxFunc (freeName : Syntax) (f : Syntax) (oix : Option Syntax) : CommandElabM Unit := do
   let c1c : Syntax := Lean.mkIdent (freeName.getId ++ "Pure")
   let c2c : Syntax := Lean.mkIdent (freeName.getId ++ "Impure")
   let cd ←
-    `(instance {ix : Type} {b : Type → Type} [Prismatic b $f] : SendableIx b (@$freeName ix) where
-        sendIx := fun v => $c2c (Prismatic.inject v) $c1c)
+    match oix with
+    | Option.none =>
+          `(instance {ix : Type} {b : Type → Type} [Prismatic b $f] : SendableIx b (@$freeName ix) where
+              sendIx := fun v => $c2c (Prismatic.inject v) $c1c)
+    | Option.some ix =>
+          `(instance             {b : Type → Type} [Prismatic b $f] : SendableIx b $freeName where
+              sendIx := fun v => $c2c (Prismatic.inject v) $c1c)
   elabCommand cd
 
+def mkInterpreterFunc (freeName : Syntax) (sumName : Syntax) (interpretName : Syntax) (oix : Option Syntax) : CommandElabM Unit := do
+  let c1c : Syntax := Lean.mkIdent (freeName.getId ++ "Pure")
+  let c2c : Syntax := Lean.mkIdent (freeName.getId ++ "Impure")
+  let c1pat ← `(matchAltExpr| | $c1c a => pure a)
+  let c2pat ← `(matchAltExpr| | $c2c v next => bind (c v) (fun xx => $interpretName c (next xx)))
+  let branches := #[c1pat,c2pat]
+  let cd ←
+    match oix with
+    | Option.none =>
+          `(def $interpretName {ix α : Type} {i : Indexer ix}  {n : Type → Type} [Monad n] (c : {z : Type} → $sumName z → n z) (m : $freeName i α) : n α :=
+              match m with $branches:matchAlt*)
+    | Option.some ix =>
+          `(def $interpretName {   α : Type} {i : Indexer $ix} {n : Type → Type} [Monad n] (c : {z : Type} → $sumName z → n z) (m : $freeName i α) : n α :=
+              match m with $branches:matchAlt*)
+  elabCommand cd
+  
 
-elab "mkFreer" freeName:ident f:ident : command => do
+def mkFreerFunc (freeName : Syntax) (f : Syntax) (oix : Option Syntax) : CommandElabM Unit := do
   let mapName : Syntax := Lean.mkIdent <| Name.mkSimple <| freeName.getId.toString ++ "mapX"
   let bindName : Syntax := Lean.mkIdent <| Name.mkSimple <| freeName.getId.toString ++ "bindX"
   let bindIxName : Syntax := Lean.mkIdent <| Name.mkSimple <| freeName.getId.toString ++ "bindXX"
   let reindexName : Syntax := Lean.mkIdent <| Name.mkSimple <| freeName.getId.toString ++ "reindexX"
-  let m1 ← `(mkFreerInductive $freeName $f)
+  let interpreterName : Syntax := Lean.mkIdent <| Name.mkSimple <| "run" ++ freeName.getId.toString
+  let m1 ← match oix with
+           | Option.none    => `(mkFreerInductive $freeName $f)
+           | Option.some ix => `(mkFreerInductiveWithIndex $freeName $f $ix)
   elabCommand m1
   let m2 ← `(mkFmap $freeName $mapName $f)
   elabCommand m2
   let m3 ← `(mkFFunctor $freeName $mapName $f)
   elabCommand m3
-  let m4 ← `(mkFMonad $freeName $bindName $f)
-  elabCommand m4
-  let m5 ← `(mkIxMonad $freeName $bindIxName $reindexName $f)
-  elabCommand m5
-  let m6 ← `(mkSendableIx $freeName $f)
-  elabCommand m6
+  mkFMonadFunc freeName bindName f oix
+  mkIxMonadFunc freeName bindIxName reindexName f oix
+  mkSendableIxFunc freeName f oix
+  mkInterpreterFunc freeName f interpreterName oix
+  /-
+  let m7 ← `(mkInterpreter $freeName $f $interpreterName)
+  elabCommand m7
+  -/
+
+elab "mkFreer" freeName:ident f:ident : command => mkFreerFunc freeName f Option.none
+elab "mkFreer" freeName:ident f:ident z:term : command => mkFreerFunc freeName f (Option.some z)
 
 /-
-mkFreerInductive SomeFreer Id
-mkFmap SomeFreer mapX Id
-mkFFunctor SomeFreer mapX Id
-mkFMonad SomeFreer bindY Id
-mkIxMonad SomeFreer bindIxY reindexIxY Id
-mkSendableIx SomeFreer Argh
--/
-
+set_option pp.rawOnError true
 mkFreer SomeFreer Argh
+mkFreer SomeFreerNat Argh Nat
 #print SomeFreer
-
+#print SomeFreerNat
+#check SomeFreer_interpret
 
 #check (do SomeFreer.Pure (); SomeFreer.Pure 4 : SomeFreer Indexer.Null Nat)
-#check (Prismatic.inject (SomeI.A 3) : Argh Nat)
-#check (send (SomeI.A 3) : SomeFreer _ _)
+#check (Prismatic.inject (EcksI.X  3 7) : Argh Nat)
+#check (send (EcksI.X 1 3) : SomeFreer _ _)
+
+
 
 open IxMonad
 
 def x {m : Indexer Nat → Type → Type 1}
-  [IxMonad m] [SendableIx SomeI m] :=
+  [IxMonad m] [SendableIx (EcksI Nat) m] :=
     checkIxDo m Nat Nat ∃>
-           (send <| SomeI.A ())
-        →→ (sendIndexed 2 (SomeI.A ()))
+           (send <| EcksI.X 1 1)
+        →→ (sendIndexed 2 (EcksI.X 22 ()))
         →→ (pure0 3)
 
 def runSome := @x SomeFreer
 
 #check runSome
 #eval getIndex runSome
-
+-/
 
 end FreerIx
