git/cruhland/lean4-axiomatic/Lean4Axiomatic/Integer/Impl/Derived/Negation.lean
@@ -1,0 +1,94 @@
+import Lean4Axiomatic.Integer.Negation
+
+namespace Lean4Axiomatic.Integer.Impl.Derived
+
+variable {ℕ : Type}
+variable [Natural ℕ]
+variable {ℤ : Type}
+variable [Equality ℤ]
+variable [Conversion ℕ ℤ]
+variable [Addition.Base ℕ ℤ]
+variable [Multiplication.Base ℕ ℤ]
+variable [Negation.Base ℕ ℤ]
+
+/--
+Zero is a left absorbing element for multiplication.
+
+**Property intuition**: A sum of zero terms should produce the empty sum, i.e.
+the additive identity, which is zero.
+
+**Proof intuition**: The only way to produce zero by itself, given the
+properties of integer addition and multiplication, is by adding a value to its
+negation. So we somehow need to obtain `0 * a + -(0 * a)` from `0 * a`. We can
+easily get `0 * a + (0 * a + -(0 * a))` from the additive identity and inverse
+properties. The key is then using associativity, distributivity, and again
+additive identity to merge the two instances of `0 * a` into one.
+-/
+def mul_absorbL {a : ℤ} : 0 * a ≃ 0 := calc
+  0 * a                      ≃ _ := Rel.symm AA.identR
+  0 * a + 0                  ≃ _ := AA.substR (Rel.symm AA.inverseR)
+  0 * a + (0 * a + -(0 * a)) ≃ _ := Rel.symm AA.assoc
+  (0 * a + 0 * a) + -(0 * a) ≃ _ := AA.substL (Rel.symm AA.distribR)
+  (0 + 0) * a + -(0 * a)     ≃ _ := AA.substL (AA.substL AA.identL)
+  0 * a + -(0 * a)           ≃ _ := AA.inverseR
+  (0 : ℤ)                    ≃ _ := Rel.refl
+
+def mul_absorbingL : AA.AbsorbingOn Hand.L (α := ℤ) 0 (· * ·) := {
+  absorb := mul_absorbL
+}
+
+local instance mul_absorbing : AA.Absorbing (α := ℤ) 0 (· * ·) := {
+  absorbingL := mul_absorbingL
+  absorbingR := AA.absorbingR_from_absorbingL mul_absorbingL
+}
+
+/--
+Negation is left-semicompatible with multiplication.
+
+**Property intuition**: Negating the sum of `b` copies of `a` should be the
+same as the sum of `b` copies of `-a`.
+
+**Proof intuition**: We're showing how negation and multiplication interact, so
+there's no preexisting property that tells us how to manipulate `-(a * b)`. The
+next best thing is to try to introduce some new terms, one of which is our
+desired result `(-a) * b`, but the other is `a * b` to cancel out `-(a * b)`.
+And it turns out those new terms have a factor of `b` in common, so we can
+produce them using distributivity and the additive inverse property.
+-/
+theorem neg_scompatL_mul {a b : ℤ} : -(a * b) ≃ (-a) * b := calc
+  -(a * b)
+    ≃ _ := Rel.symm AA.identL
+  0 + -(a * b)
+    ≃ _ := AA.substL (Rel.symm AA.absorbL)
+  0 * b + -(a * b)
+    ≃ _ := AA.substL (AA.substL (Rel.symm AA.inverseL))
+  (-a + a) * b + -(a * b)
+    ≃ _ := AA.substL AA.distribR
+  (-a * b + a * b) + -(a * b)
+    ≃ _ := AA.assoc
+  (-a) * b + (a * b + -(a * b))
+    ≃ _ := AA.substR AA.inverseR
+  (-a) * b + 0
+    ≃ _ := AA.identR
+  (-a) * b
+    ≃ _ := Rel.refl
+
+def neg_semicompatibleL_mul
+    : AA.SemicompatibleOn Hand.L (α := ℤ) (-·) (· * ·)
+    := {
+  scompat := neg_scompatL_mul
+}
+
+def neg_semicompatible_mul : AA.Semicompatible (α := ℤ) (-·) (· * ·) := {
+  semicompatibleL :=
+    neg_semicompatibleL_mul
+  semicompatibleR :=
+    AA.semicompatibleR_from_semicompatibleL neg_semicompatibleL_mul
+}
+
+def negation_derived : Negation.Derived ℕ ℤ := {
+  mul_absorbing := mul_absorbing
+  neg_semicompatible_mul := neg_semicompatible_mul
+}
+
+end Lean4Axiomatic.Integer.Impl.Derived
